Here is a similar problem with the step-by-step solution.

## ‚úçÔ∏è Problem Statement

Find the power series representation for the function $f(x) = \frac{x^2}{(1 - 2x)^2}$ and determine the radius of convergence.

---

## üõ†Ô∏è Step-by-Step Solution

The goal is to manipulate the base geometric series formula, $\frac{1}{1-r} = \sum_{n=0}^\infty r^n$, to match the given function.

### Step 1: Start with the Base Geometric Series

We begin with the base function related to the denominator:
$$\frac{1}{1-x} = \sum_{n=0}^\infty x^n$$
This series is valid for $|x| < 1$, so the radius of convergence is $R=1$.

### Step 2: Substitute to Match the Denominator

The desired denominator is $(1 - 2x)^2$, so we first need to get $1 - 2x$ in the base of the series. We substitute $\mathbf{2x}$ for $x$ in the series from Step 1:
$$\frac{1}{1 - 2x} = \sum_{n=0}^\infty (2x)^n = \sum_{n=0}^\infty 2^n x^n$$
This series is valid when $|2x| < 1$, which means $|x| < \frac{1}{2}$. The radius of convergence is $\mathbf{R = \frac{1}{2}}$.

### Step 3: Differentiate to Get the Square

The function contains the term $\frac{1}{(1-2x)^2}$. Recall that the derivative of $\frac{1}{1-u}$ is $\frac{1}{(1-u)^2}$.
We differentiate both sides of the equation from Step 2 with respect to $x$:

**Left Side (Function):**
$$\frac{d}{dx} \left[ \frac{1}{1 - 2x} \right] = \frac{-(-2)}{(1 - 2x)^2} = \frac{2}{(1 - 2x)^2}$$

**Right Side (Series):**
$$\frac{d}{dx} \left[ \sum_{n=0}^\infty 2^n x^n \right] = \sum_{n=1}^\infty \frac{d}{dx} \left[ 2^n x^n \right] = \sum_{n=1}^\infty \mathbf{n 2^n x^{n-1}}$$
*Note: The summation starts at $n=1$ because the $n=0$ term is a constant, which differentiates to $0$.*

Equating the results gives:
$$\frac{2}{(1 - 2x)^2} = \sum_{n=1}^\infty n 2^n x^{n-1}$$

### Step 4: Isolate the Denominator Term $\frac{1}{(1-2x)^2}$

We divide both sides of the equation from Step 3 by $\mathbf{2}$:
$$\frac{1}{(1 - 2x)^2} = \frac{1}{2} \sum_{n=1}^\infty n 2^n x^{n-1} = \sum_{n=1}^\infty n \frac{2^n}{2} x^{n-1} = \sum_{n=1}^\infty n \mathbf{2^{n-1}} x^{n-1}$$

### Step 5: Multiply by the Numerator $x^2$

The original function is $f(x) = x^2 \cdot \frac{1}{(1 - 2x)^2}$. We multiply the series from Step 4 by $\mathbf{x^2}$:
$$f(x) = x^2 \sum_{n=1}^\infty n 2^{n-1} x^{n-1}$$
$$f(x) = \sum_{n=1}^\infty n 2^{n-1} \cdot x^2 \cdot x^{n-1}$$
Using the exponent rule $x^a x^b = x^{a+b}$:
$$f(x) = \sum_{n=1}^\infty n 2^{n-1} \mathbf{x^{n+1}}$$

### Final Answer: Power Series and Radius of Convergence

The power series representation for $f(x) = \frac{x^2}{(1 - 2x)^2}$ is:
$$f(x) = \sum_{n=1}^\infty n 2^{n-1} x^{n+1}$$

The radius of convergence $\mathbf{R}$ remains the same as the series used in the differentiation step (Step 2), which is $\mathbf{R = \frac{1}{2}}$.
