

## üõ†Ô∏è Step-by-Step Guide: Power Series Representation

**Function:** $f(x) = \frac{x^2 + x}{(1 - x)^3}$

### Phase A: Build the Denominator $\left(\frac{1}{(1-x)^3}\right)$

1.  **Start with the Base Series:** Write the known geometric series formula for $g(x) = \frac{1}{1 - x}$, ensuring you use the series notation and the first few expanded terms.
    $$\frac{1}{1 - x} = \sum_{n=0}^{\infty} x^n$$
2.  **Determine Required Derivatives:** Calculate the derivative of the base function $\frac{1}{1-x}$ until the denominator is raised to the power you need (in this case, 3).
    * $\frac{d}{dx} \left(\frac{1}{1-x}\right) = \frac{1}{(1-x)^2}$ (First Derivative)
    * $\frac{d^2}{dx^2} \left(\frac{1}{1-x}\right) = \frac{2}{(1-x)^3}$ (Second Derivative)
3.  **Apply Derivatives to the Series:** Differentiate the series from Step 1 **term-by-term** two times. *Crucially, remember that differentiation shifts the starting index.*
    * $g'(x) = \sum_{n=1}^{\infty} \frac{d}{dx} (x^n) = \sum_{n=1}^{\infty} n x^{n-1}$
    * $g''(x) = \sum_{n=2}^{\infty} \frac{d}{dx} (n x^{n-1}) = \sum_{n=2}^{\infty} n(n-1) x^{n-2}$
4.  **Isolate the Target Denominator:** Solve the relationship from Step 2 to isolate the target fraction $\frac{1}{(1-x)^3}$. Then, apply that same operation to the final series obtained in Step 3.
    $$\frac{1}{(1-x)^3} = \frac{1}{2} \cdot g''(x) = \frac{1}{2} \sum_{n=2}^{\infty} n(n-1) x^{n-2}$$

### Phase B: Incorporate the Numerator $\left(x^2 + x\right)$

5.  **Multiply by the Numerator Terms:** Substitute the series expression found in Step 4 back into the original function $f(x)$:
    $$f(x) = (x^2 + x) \cdot \left[ \frac{1}{2} \sum_{n=2}^{\infty} n(n-1) x^{n-2} \right]$$
6.  **Distribute the Powers of $x$:** Distribute the $x^2$ and $x$ terms into the summation. This means adding the exponents inside the summation:
    * $x^2 \cdot x^{n-2} = x^{n-2+2} = x^n$
    * $x \cdot x^{n-2} = x^{n-2+1} = x^{n-1}$
7.  **Split and Simplify:** You will now have two separate series.
    $$f(x) = \frac{1}{2} \sum_{n=2}^{\infty} n(n-1) x^{n} + \frac{1}{2} \sum_{n=2}^{\infty} n(n-1) x^{n-1}$$

### Phase C: Combine the Series (Optional but Best Practice)

8.  **Index Adjustment:** Adjust the index of the second series (the one with $x^{n-1}$) so that its power is also $x^n$.
    * Let $k = n-1$ (which means $n = k+1$).
    * When $n=2$, $k=1$.
    * The second series becomes: $\frac{1}{2} \sum_{k=1}^{\infty} (k+1)k x^{k}$
9.  **Combine the Series:** Since both series now have the power $x^n$ (or $x^k$) and you can choose the higher starting index (2) for $n$ to avoid having to split out terms, you can combine the coefficients.

---

**Now that you have this clear map, let's start with Step 3:**

You already correctly stated the first part of the derivative, but let's formalize the **Second Derivative**.

**Your Task (Step 3):**

Given the First Derivative Series $g'(x) = \sum_{n=1}^{\infty} n x^{n-1}$, calculate the **Second Derivative Series**, $g''(x)$.

1.  Write the resulting **general term** of the $g''(x)$ series.
2.  Write the new **starting index** (where $n$ begins).

Go ahead and state the series for $g''(x)$!
